> Use the definition of functional dependency to argue that each of Armstrong's axioms
> (reflexivity, augmentation, and transitivity) is sound. 

--------------------------------

* **Reflexivity rule** If $\alpha$ is a set of attributes and $\beta \subseteq \alpha$, then $\alpha \rightarrow \beta$ holds.

Let $r(R)$ be a relation schema. Let $\beta \subseteq \alpha \subseteq R$. Let $t_1$ and $t_2$ be 
two tuples in $r$ such that: 
$$
t_1[\alpha] = t_2[\alpha]
$$

Let $x$ be any attribute in $\beta$. Then the value of the attribute $x$ in $t_1$ is the same as the 
value of the attribute $x$ in $t_2$ (since $x \in \beta \text{ implies } x \in \alpha$).Thus,  
$$
t_1[\beta] = t_2[\beta]
$$

Therefore, by definition of functional dependency, $\alpha \rightarrow \beta$ holds.

* **Augmentation rule** If $\alpha \rightarrow \beta$ holds and $\gamma$ is a set of attributes, then 
$\gamma\alpha \rightarrow \gamma\beta$ holds.

Let $r(R)$ be a relation schema and  $\alpha \rightarrow \beta$
holds on $r(R)$. Let $\gamma \subseteq R$. Let $t_1$ and $t_2$ be two tuples in $r$ such that: 
$$
t_1[\gamma\alpha] = t_2[\gamma\alpha]
$$

Let $x$ be an attribute in $\gamma\beta$. Then either $x \in \gamma$ or $x \in \beta$. 
Suppose $x \in \gamma$. Then the value of the attribute $x$ in $t_1$ is the same as the 
value of the attribute $x$ in $t_2$ (since $x \in \gamma\alpha$ and we assumed that 
$t_1[\gamma\alpha] = t_2[\gamma\alpha]$). Now suppose $x \in \beta$. Then the value of the 
attribute $x$ in $t_1$ is the same as the value of the attribute $x$ in $t_2$ (this is 
because of the functional dependency $\alpha \rightarrow \beta$ that holds on $r(R)$ and 
the fact that $t_1$ and $t_2$ have the same values on all attributes in $\alpha$ due to 
the condition $t_1[\gamma\alpha] = t_2[\gamma\alpha]$). Since $x$ was arbitrary in $\gamma\beta$
we conclude that 
$$
t_1[\gamma\beta] = t_2[\gamma\beta]
$$
Thus $\gamma\alpha \rightarrow \gamma\beta$ holds.

* **Transitivity rule** If $\alpha \rightarrow \beta$ holds and $\beta \rightarrow \gamma$ holds, then 
$\alpha \rightarrow \gamma$.

Let $r(R)$ be a relation schema and the set of functional dependencies $F = \{\alpha \rightarrow \beta, \beta \rightarrow \gamma\}$
holds on $r(R)$. Let $t_1$ and $t_2$ be two tuples in $r$ such that: 
$$
t_1[\alpha] = t_2[\alpha]
$$
Since we know that $\alpha \rightarrow \beta$ holds on $r(R)$, it follows from the definition of functional dependency
that: 
$$
t_1[\beta] = t_2[\beta]
$$
Then, since we know that $\beta \rightarrow \gamma$ holds on $r(R)$, it follows from the definition of functional dependency
that: 
$$
t_1[\gamma] = t_2[\gamma]
$$
Therefore, we have shown that, whenever $t_1$ and $t_2$ are tuples such that $t_1[\alpha] = t_2[\alpha]$, it must be 
that $t_1[\gamma] = t_2[\gamma]$. But that is exactly the definition of $\alpha \rightarrow \gamma$